pcuic/theories/PCUICTyping.v
@@ -34,7 +34,7 @@ Fixpoint isArity T :=
   | _ => false
   end.
 
-Definition type_of_constructor mdecl (cdecl : constructor_body) (c : inductive * nat) (u : list Level.t) :=
+Definition type_of_constructor mdecl (cdecl : constructor_body) (c : inductive * nat) (u : Instance.t) :=
   let mind := inductive_mind (fst c) in
   subst0 (inds mind u mdecl.(ind_bodies)) (subst_instance u (cstr_type cdecl)).
 
@@ -189,10 +189,10 @@ Variant primitive_typing_hyps `{checker_flags}
 Derive Signature for primitive_typing_hyps.
 
 Equations prim_type (p : prim_val term) (cst : kername) : term :=
-prim_type (primInt; _) cst := tConst cst [];
-prim_type (primFloat; _) cst := tConst cst [];
-prim_type (primString; _) cst := tConst cst [];
-prim_type (primArray; primArrayModel a) cst := tApp (tConst cst [a.(array_level)]) a.(array_type).
+prim_type (primInt; _) cst := tConst cst Instance.empty;
+prim_type (primFloat; _) cst := tConst cst Instance.empty;
+prim_type (primString; _) cst := tConst cst Instance.empty;
+prim_type (primArray; primArrayModel a) cst := tApp (tConst cst (Instance.make [] [a.(array_level)])) a.(array_type).
 Transparent prim_type.
 
 Inductive typing `{checker_flags} (Σ : global_env_ext) (Γ : context) : term -> term -> Type :=
